Graph/IRGraph.thy
@@ -55,6 +55,16 @@ lift_definition irgraph :: "(ID \<times> (IRNode \<times> Stamp)) list \<Rightar
   is "map_of \<circ> no_node"
   by (simp add: finite_dom_map_of)
 
+definition as_set :: "IRGraph \<Rightarrow> (ID \<times> (IRNode \<times> Stamp)) set" where
+  "as_set g = {(n, kind g n, stamp g n) | n . n \<in> ids g}"
+
+definition domain_subtraction :: "'a set \<Rightarrow> ('a \<times> 'b) set \<Rightarrow> ('a \<times> 'b) set"
+  (infix "\<unlhd>" 30) where
+  "domain_subtraction s r = {(x, y) . (x, y) \<in> r \<and> x \<notin> s}"
+
+notation (latex)
+  domain_subtraction ("_ \<^latex>\<open>$\\ndres$\<close> _")
+
 (* Theories are required for code generation to work *)
 code_datatype irgraph
 
